# 4.1 Fundamental groups

## 4.1.1 Basic ideas

We say a loop $\alpha$ is homotopic to $\beta$ if $\alpha$ can be obtained from $\beta$ by a continuous deformation. "Homotopic to" is an equivalence relation, the equivalence class of which is called the homotopy class. The set of homotopy classes is endowed with a group structure called the **fundamental group**. *(No formal definition has been given yet in this section)*

## 4.1.2 Paths and loops

> **Definition 4.1.**  Let $X$ be a topological space and let $I=[0,1]$.  A continuous map $\alpha\ :I\rightarrow X$ is called a **path** with an initial point $x_0$ and an end point $x_1$ if $\alpha(0)=x_0$ and $\alpha(1)=x_1$. If $\alpha(0)=\alpha(1)=x_0$, the path is called a loop with base point $x_0$ (or a loop at $x_0$).

For $x\in X$, a **constant path** $c_x\ : I\rightarrow X$ is defined by $c_x (s) =x,  s\in I$,  A constant path is also a constant loop.

> **Definition 4.2.** Let $\alpha, \beta\ : I\rightarrow X$ be paths such that $\alpha(1)=\beta(0)$. The product of $\alpha$ and $\beta$, denoted by $\alpha\*\beta$, is a path in $X$ defined by
> $$\alpha\*\beta(s)=\begin{cases}
    \alpha(2s) &0\le s\le\frac{1}{2}\\\\
    \beta(2s-1)&\frac{1}{2}\le s\le 1
\end{cases}$$ 

$\alpha*\beta$ is a continuous map from $I$ to $X$.<mark>(rigorous proof?)</mark>

> **Definition 4.3.** Let $\alpha\ ; I\rightarrow X$ be a path from $x_0$ to $x_1$. The inverse path $\alpha^{-1}$ of $\alpha$ is defined by 
> $$\alpha^{-1}(s)\equiv \alpha(1-s)\quad s\in I$$

## 4.1.3 Homotopy

> **Definition 4.4.** Let $\alpha, \beta\ : I\rightarrow X$ be loops at $x_0$. They are said to be homotopic, written as $\alpha \sim \beta$, if there exists a continuous map $F\ : I\times I\rightarrow X$ such that
> $$\begin{gather}
    F(s,0)=\alpha(s),\quad F(s,1)=\beta(s)\quad \forall s\in I\\\\
    F(0,t)=F(1,t)=x_0\quad \forall t\in I
\end{gather}$$
>The connecting map $F$ is called a **homotopy** between $\alpha$ and $\beta$.

> **Proposition 4.1.** The relation $\alpha\sim\beta$ is an equivalence relation.
> 
> **Proof.** 
> 1. Reflectivity: Choose the homotopy to be $F(s,t)=\alpha(s)$ for any $t\in I$.
> 2. Symmetry: Let $\alpha\sim\beta$ with the homotopy $F(s,t)$. Then $\beta\sim\alpha$ with the homotopy $F'(s,t)=F(s,1-t)$.
> 3. Transitivity: Let $\alpha\sim\beta$ with the homotopy $F(s,t)$ and $\beta\in\gamma$ with the homotopy $G(s,t)$. Then $\alpha\sim\gamma$ with the homotopy:
> $$H(s,t)=\begin{cases}
    F(s,2t)&0\le t\le\frac{1}{2}\\\\
    G(s,2t-1)& \frac{1}{2}\le t\le 1.
\end{cases}$$


## 4.1.4 Fundamental groups

The equivalence class of loops is denoted by $[a]$ and is called the **homotopy class** of $\alpha$.

> **Definition 4.5.** Let $X$ be a topological space. The set of homotopy classes of loops at $x_0 \in X$ is denoted by $\pi_1 (X,x_0)$ and is called the **fundamental group**(or **the first homotopy group**) of $X$ at $x_0$. The product of homotopy classes $[\alpha]$ and $[\beta]$ is defined by
> $$[\alpha]\*[\beta]=[\alpha\*\beta]$$

> **Lemma 4.1.** The product of homotopy classes is independent of the representative, that is, if $\alpha\sim\alpha'$ and $\beta\sim\beta'$, then $\alpha\*\beta\sim\alpha' \* \beta'$.
>  **Proof** Let $F(s,t)$ be a homotopy between $\alpha$ and $\alpha'$ and $G(s,t)$ be a homotopy between $\beta$ and $\beta'$. Then $\alpha\*\beta\sim\alpha'\sim\beta'$ with the homotopy
> $$H(s,t)=\begin{cases}
    F(2s,t)&0\le s\le \frac{1}{2}\\\\
    G(2s-1,t)&\frac{1}{2}\le s\le 1
\end{cases}$$

> **Theorem 4.1.** The fundamental group is a group. Namely, if $\alpha, \beta,\dots$ are loops at $x\in X$, the follwoing group properties are satisfied:
> 1. $([\alpha]\*[\beta])\*[\gamma]=[\alpha]\*([\beta]*[\gamma])$
> 2. $[\alpha]\*[c_x]=[\alpha]$ and $[c_x]\*[\alpha]=[\alpha]$ (unit element)
> 3. $[\alpha]*[\alpha^{-1}]=[c_x]$, hence $[\alpha]^{-1}=[\alpha^{-1}]$ (inverse)
>
>**Proof** 
>1. $(\alpha\*\beta)\*\gamma\sim\alpha\*(\beta\*\gamma)$ with the homotopy
>$$F(s,t)=\begin{cases}
    \alpha\left(\frac{4s}{1+t}\right)&0\le s\le \frac{1+t}{4}\\\\
    \beta(4s-t-1)&\frac{1+t}{4}\le s\le \frac{2+t}{4}\\\\
    \gamma\left(\frac{4s-t-2}{2-t}\right)& \frac{2+t}{4}\le s\le 1
\end{cases}$$
> Thus, we denote $(\alpha\*\beta)\*\gamma$ or $\alpha\*(\beta\*\gamma)$ by $[\alpha\*\beta\*\gamma]$
>
>2. $(\alpha\* c_x)\sim\alpha$ with the homotopy
>$$F(s,t)=\begin{cases}
    \alpha\left(\frac{2s}{1+t}\right)& 0\le s\le \frac{t+1}{2}\\\\
    x & \frac{t+1}{2}\le s\le 1.
\end{cases}$$
> Similarly, $(c_x\*\alpha)\sim\alpha$ with the homotopy 
> $$F(s,t)=\begin{cases}
    x & 0\le s\le \frac{1-t}{2}\\\\
    \alpha\left(\frac{2s-1+t}{1+t}\right) & \frac{1-t}{2}\le s\le 1.
\end{cases}$$
> So, $[\alpha]\*[c_x]=[\alpha]=[c_x]\*[\alpha]$
>
>3. Define a map $F\ : I\times I\rightarrow X$ by:
>$$F(x,y)=\begin{cases}
    \alpha(2s(1-t))& 0\le s\le \frac{1}{2}\\\\
    \alpha(2(1-s)(1-t))& \frac{1}{2}\le s\le 1.
\end{cases}$$
>So $F(s,0)=\alpha\*\alpha^{-1}$ and $F(s,1)=c_x$, hence
>$$[\alpha\*\alpha^{-1}]=[\alpha]\*[\alpha^{-1}]=[c_x].$$
>Thus, $[\alpha^{-1}]=[\alpha]^{-1}$