# 5.4 Differential forms

## 5.4.0 Symmetry operation
Consider a $(0,r)$ form tensor $\omega\in{{\tau}_{r,p}}^0(M) $, them we can define the symmetrizer and anti-symmetrizer operate.
> **Definition 5.4.0** For symmetrizer we have: $$\omega_{(\mu_1\mu_2...\mu_r)}=\frac{1}{r!}\Sigma_{\pi}\omega_{\mu_{\pi(1)}...\mu_{\pi(r)}}$$ and for anti-symmetrizer we have: $$\omega_{[\mu_1\mu_2...\mu_r]}=\frac{1}{r!}\Sigma_{\pi}\delta_{\pi}\omega_{\mu_{\pi(1)}...\mu_{\pi(r)}}$$, where $\delta_{\pi}=\pm 1$ if it is even permutations or odd permutations.

## 5.4.1 Def of forms
> **Def 5.4.1** A differential form of order r or an r-form is a totally anti-symmetric tensor of type $(0,r)$. That is: $$\omega_{\mu_1\mu_2...\mu_r}=\omega_{[\mu_1\mu_2...\mu_r]}$$.
> **Def 5.4.2** Let us define the wedge product $\wedge$ of r one-form by the totally anti-symmetric tensor product: $$dx^{\mu_1}\wedge...\wedge dx^{\mu_r}=\Sigma_{\pi}\delta_{\pi}dx^{\mu_{\pi(1)}}\wedge...\wedge dx^{\mu_{\pi(r)}}$$. For example: $$dx^{\mu}\wedge dx^{\nu}=dx^{\mu}\bigotimes dx^{\nu}-dx^{\nu}\bigotimes dx^{\mu}$$.
It is readily verified that the wedge product satisfies the following:
(i) $dx^{\mu_1}\wedge...\wedge dx^{\mu_r}=0$ if some index $\mu$ appears at least twice.
(ii)$dx^{\mu_1}\wedge...\wedge dx^{\mu_r}=\delta_{\pi}dx^{\mu_{\pi(1)}}\wedge...\wedge dx^{\mu_{\pi(r)}}$
(iii)$dx^{\mu_1}\wedge...\wedge dx^{\mu_r}$ is liner in each $dx^{\mu}$
> **Def 5.4.3** ${\Omega_p}^r(M)$ is a vector space of r-form at p point.
$\omega\in{\Omega_p}^r(M)$ can be expanded as: $$\omega=\frac{1}{r!}\omega_{\mu_1...\mu_r}dx^{\mu_1}\wedge...\wedge dx^{\mu_r}=\omega_{[\mu_1...\mu_r]}$$. So we find that any tensor $\omega_{\mu\nu}$ can be witten: $$\omega_{\mu\nu}=\sigma_{\mu\nu}+\alpha_{\mu\nu}=\omega_{(\mu\nu)}+\omega_{[\mu\nu]}$$.

Prove that $dim {\Omega_r}^r(M)={C_m}^r$ :
> Prove: For $\forall\quad r,m,r\leq m$, we have:
> $$\omega_{\mu_1...\mu_r}=\Sigma_{C}\omega_{\mu_1...\mu_r}{(e^{\mu_{1}})}_{a_{1}}\wedge...\wedge {(e^{\mu_1})}_{a_{r}}$$, where $\\{{(e^1)}_{a}...{(e^m)}_a\\}$ is a basis of ${V_p}^{*}$. $\omega_{\mu_1...\mu_r}$ is the component of $\omega$ in the basis of $F_V(0,l)$ with this basis: $$\omega_{\mu_1...\mu_r}=\omega_{a_1...a_r}(e_{\mu_1})^{a_1}...(e_{\mu_r})^{a_r}$$. $\Sigma_C$ is the sum of r combinations of m numbers, Q.E.D.
And we can get:
> $$dim {\Omega_p}^r(M)={\Omega_p}^{m-r}(M)$$
> $${\Omega_p}^r(M)\backsimeq{\Omega_p}^{m-r}(M)$$
## 5.4.2 Exterior product
> **Def5.4.4** ${\Omega_p}^q(M)\times {\Omega_p}^r(M)\to {\Omega_p}^{q+r}(M)$. 
Let $\omega\in {\Omega_p}^q(M)$, $\xi\in {\Omega_p}^r(M)$, them the $(q+r)$ form is defined by:
> $$(\omega\wedge\xi)(V_1...V_{q+r})=\frac{(q+r)!}{q!r!}\Sigma_{\pi}\delta_{\pi}\omega(V_{\pi(1)}...V_{\pi(q)})\xi(V_{\pi(q+1)}...V_{\pi(q+r)})=\frac{(q+r)!}{q!r!}\omega_{[a_1...a_r\mu_{b_1...b_r}]}$$.
Where $V_i\in T_p(M)$, if $q+r>m$, $\omega\wedge\xi=0$.
We define an algebra:
> $${\Omega_p}^{*}(M)={\Omega_p}^0(M)\bigoplus...\bigoplus{\Omega_p}^m(m)$$.
> ${\Omega_p}^{*}(M)$ 为p处所有微分形式的集合，且对外积封闭。
我们可以在流形M上每一点给出r形式，M上光滑r形式空间写为 ${\Omega}^r(M)$ . 有此表。
## 5.4.3 Exterior derivatives
> **Def 5.4.5** The exterior derivative $d_r$ is a map $\Omega^r(M)\to\Omega^{r+1}(M)$ whose action on an r-form
> $$\omega=\frac{1}{r!}\omega_{\mu_1...\mu_r}dx^{\mu_1}\wedge...\wedge dx^{\mu_r}$$
is defined by
> $$d_r\omega=\frac{1}{r!}(\frac{\partial}{\partial x^{\nu}}\omega_{\mu_1...\mu_r})dx^{\nu}\wedge dx^{\mu_1}\wedge...\wedge dx^{\mu_r}$$
Example:...
By the way:
> $$\omega\wedge\xi=(-1)^{rq}(\xi\wedge\omega)$$
A useful exterior derivative:
> $$X[\omega(Y)]-Y[\omega(X)]-\omega([X.Y])=\frac{\partial\omega_{\mu}}{\partial x^{\nu}}(X^{\nu}Y^{\mu}-X^{\mu}Y^{\nu})=d\omega(X,Y)$$
> For $\omega\in\Omega^r(M)$:
> $$d\omega(X_1...X_{r+1}) =\sum_{i=1}^r(-1)^{i+j}X_i\omega(X_1...\hat{X_i}...X_{r+1})+\sum_{i<j}(-1)^{i+j}\omega([X_i,X_j],X_1...\hat{X_i}...\hat{X_j}..X_{r+1})$$
Prove: $d^2=0(d_{r+1}d_r=0)$
> We take $\omega\in\Omega^r(M)$
> $$d^2\omega=\frac{1}{r!}\frac{{\partial}^2\omega_{\mu_1...\mu_r}}{\partial x^{\lambda}\partial x^{\nu}}dx^{\lambda}\wedge dx^{\nu}\wedge dx^{\mu_1}...dx^{\mu_r}$$
Since $\frac{{\partial}^2\omega_{\mu_1...\mu_r}}{\partial x^{\lambda}\partial x^{\nu}}$ is symmetric with respect to $\lambda$ and $\nu$ while $dx^{\lambda}\wedge dx^{\nu}$ is anti-symmetric, so $d^2\omega=0$.


In sec5.2 we defined a pull back map $f^{\star}$ : ${T_{f(p)}(M)}^{\star}\to{T_p(M)}^{\star}$, $f^{\star}$ can be expanded to a $(0,r)$ form tensor.
> **Def 5.4.6** Let $\omega\in\Omega^{r}(M)$, $f:M\to N$, in each $f(P)\in N$, $f$ induces the pullback $f^{\star}: {\Omega_{f(p)}}^{\star}N\to{\Omega_{p}}^{r}M$ by:
> $$(f^{\star}\omega)(X_1...X_r)=\omega(f_{\star}X_1...f_{\star}X_r)$$
> where $X_i\in T_{p}(M)$ and $f_{\star}$ is the differential map $T_{p}M\to T_{f(p)}N$.
> **Def 5.4.7** de Rham complex:
> $$0\stackre{i}{\longrightarrow}\Omega^{0}(M)\stackre{d_{0}}\Omega^{1}(M)\stackre{d_{1}}\cdot\cdot\cdot\stackre{d_{m-2}}\Omega^{m-1}(M)\stackre{d_{m-1}}\Omega^{m}(M)\stackre{d_m}0$$
> where i is the inclusion map $0\hookrightarrow\Omega^{0}(M)$. 

> **Def 5.4.8** $\omega\in\Omega^{r}(M)$ if $d \omega=0$, then $\omega$ is closed. If exist $l-1$-form field $\mu$ satisfy $\omega=d\mu$, $\omega$ is exact.

## 5.4.4 Interior product and Lie derivative of forms
> **Def 5.4.8** Map $i_X:\Omega^{r}(M)\to\Omega^{r-1}(M)$, $X\in\chi(M)$
> For $\omega\in\Omega^{r}(M)$, we define:
> $$i_X\omega(X_1...X_{r-1})=\omega(X,X_1...X_{r-1})$$
> For $X=X^{\mu}\frac{\partial}{\partial x^{\mu}}$, $\omega=\frac{1}{r!}\omega_{\mu_{1}...\mu{r}}dx^{\mu_1}\wedge...\wedge dx^{\mu_{r}}$, then we have
> $$i_X\omega=\farc{1}{(r-1)!}X^{\nu}\omega_{\nu\mu_2...\mu_r}dx^{\mu_2}\wedge...\wedge dx^{\mu_r}=\frac{1}{r!}\sum_{s=1}^{r}X^{\mu_s}\omega_{\mu_1...\mu_s...\mu_r}(-1)^{s-1}dx^{\mu_1}\wedge...\wedge\hat{dx^{\mu_s}}\wedge...\wedge dx^{\mu_r}
> Example: $$i_{e_{x}}(dx\wedge dy)=dy$$

The Lie derivative of a form is most neatly written with the interior product. Let $\omega=\omega_{\mu}dx^{\mu}$ be a one-form. Consider the combination:
> $$(di_X+i_Xd)\omega=d(X^{\mu}\omega_{\mu})+i_X[\frac{1}{2}(\partial_{\mu}\omega_{\nu}-\partial_{\nu}\omega_{\mu})dx^{\mu}\wedge dx^{\nu}]=(\omega_{\mu}\partial_{\nu}X^{\mu}+X^{\mu}\partial_{\mu}\omega_{\nu})dx^{\nu}$$
> $$\mathcal{L_{X}}\omega=(di_X+i_Xd)\omega$$












